\begin{proof}[of Lemma \ref{mlem:LaplaceTransformOfDerivatives}]
    We start by induction. For $n=1$ using partial integration we have
    \[
        (\mcL f)(s) = \int_{\R_{>0}} f'(t)\cdot e^{-st}\;\uplambda(dt) = \nsqbra{
            f\cdot e^{-s\cdot}
        }_0^\infty - \int_{\R_{>0}}f(t)\cdot \dv{t}e^{-st}\;\uplambda(dt).
    \]
    Because of $\lim_{x\to\infty}f(x)\cdot e^{-sx} = 0$ and $f(0)\cdot e^0 = f(0)$, as well as $\dv{t}e^{-st} = -s\cdot e^{-st}$ we therefore get
    \[
        (\mcL f)(s) = -f(0) \cdot 1 + s\cdot\int_{\R_{>0}}f(t)\cdot e^{-st}\;\uplambda(dt) = -f(0) + s\cdot\mcL f(s).    
    \] 
    For the induction step we assume the statement to hold for $n\in\N$ and show it for $n+1$. By again partially integrating we find
    \[
        (\mcL f^{(n+1)})(s) = \int_{\R_{>0}}f^{(n+1)}(t)\cdot e^{-st}\;\uplambda(dt) = \nsqbra{
            f^{(n)}\cdot e^{-s\cdot}
        }
        _0^\infty - \int_{\R_{>0}}f^{(n)}(t)\cdot \dv{t}e^{-st}\;\uplambda(dt).
    \]
    As discussed above we see $[f^{(n)}\cdot e^{-s\cdot}]_0^\infty = -f^{(n)}(0)$, which gives
    \[
        (\mcL f^{(n+1)})(s) = -f^{(n)}(0) + s\cdot\mcL f^{(n)}(s).
    \]
    By the induction hypothesis we can insert the expression for $\mcL f^{(n)}(s)$ and obtain
    \begin{align*}
        (\mcL f^{(n+1)})(s) &= -f^{(n)}(0) + s\cdot\nbra{
            s^n\cdot(\mcL f)(s) - \sum_{k=0}^{n-1}s^{n-1-k}\cdot f^{(k)}(0)
        } \\
        &= s^{n+1}\cdot(\mcL f)(s) - \sum_{k=0}^{n}s^{n-k}\cdot f^{(k)}(0).
    \end{align*}
    This concludes the proof.
\end{proof}
