\begin{mdef}{The Propagator}{Propagator}
    % Sei $f\in\mcS(\R^d)$ und $\rho_*\in\R$. Dann definieren wir den \textit{freien Propagator} $G_0:\R^d\times\C\to\R$ durch
    Let $f\in\mcS(\R^d)$ and $\rho_*\in\R$, then we define the \textit{free} or \emph{bare propagator} $G_0:\R^d\times\C\to\R$ by
    \[
        G:(p,z)\mapsto \frac{1}{z - \rho_*\cdot\bbra{\hat f(0) - \hat f(p)}}.
    \]
    The mapping $p\mapsto \rho_*\cdot\bbra{\hat f(0) - \hat f(p)}$ further describes the \textit{bare dispersion relation}.
    % Dabei beschreibt $p\mapsto \rho_*\cdot\bbra{\hat f(0) - \hat f(p)}$ die \textit{Dispersion}.
\end{mdef}